Utils.v
@@ -1,3 +1,9 @@
+From Coq Require Import
+     List
+     Relations.
+Import ListNotations.
+
+(** General purpose tactics **)
 Ltac inv H := inversion H; subst; clear H.
 
 Ltac flatten_goal :=
@@ -15,3 +21,142 @@ Ltac flatten_all :=
   | h: context[match ?x with | _ => _ end] |- _ => let Heq := fresh "Heq" in destruct x eqn:Heq
   | |- context[match ?x with | _ => _ end] => let Heq := fresh "Heq" in destruct x eqn:Heq
   end.
+
+(****************************** Lists ******************************)
+
+Inductive prefix {A: Type}: relation (list A) :=
+| Nil_Prefix: forall l, prefix [] l
+| Cons_Prefix: forall l x l', prefix l l' -> prefix (x :: l) (x :: l').
+Hint Constructors prefix.
+Infix "⊑" := prefix (at level 40).
+
+Infix "∈" := In (at level 40).
+
+Definition snoc {A: Type} (l: list A) a: list A := l ++ [a].
+
+Inductive snoc_view {A: Type}: list A -> Type :=
+| Nil: snoc_view nil
+| Snoc: forall xs x, snoc_view (snoc xs x).
+
+Fixpoint view {X: Type} (xs: list X): snoc_view xs :=
+  match xs with
+  | [] => Nil
+  | x :: xs =>
+    match view xs with
+    | Nil => Snoc [] x
+    | Snoc ys y => Snoc (x::ys) y
+    end
+  end.
+
+Lemma snoc_not_nil_l: forall {A: Type} (xs: list A) x, [] = snoc xs x -> False.
+Proof.
+  intros ? xs ? abs; destruct xs; inv abs.
+Qed.
+
+Lemma snoc_not_nil_r: forall {A: Type} (xs: list A) x, snoc xs x = [] -> False.
+Proof.
+  intros ? xs ? abs; destruct xs; inv abs.
+Qed.
+Hint Resolve snoc_not_nil_l snoc_not_nil_r.
+
+Lemma snoc_inj : forall {A: Type} (xs ys: list A) x y
+                   (EQ: snoc xs x = snoc ys y),
+    xs = ys /\ x = y.
+Proof.
+  induction xs as [| x' xs IH]; cbn; intros.
+  - destruct ys as [| ys y']; [inv EQ; auto |].
+    inv EQ.
+    exfalso; eauto.
+  - destruct ys as [| ys y']; eauto; cbn in *.
+    + destruct xs; inv EQ; exfalso; eauto. 
+    + inv EQ; edestruct IH; eauto; subst; auto.
+Qed.
+
+Ltac snoc_inv H :=
+  apply snoc_inj in H; destruct H; subst; clear H.
+
+Lemma snoc_inv: forall {X: Type} (xs: list X),
+    xs = [] \/ exists xs' x, xs = snoc xs' x.
+Proof.
+  induction xs as [| x xs IH] using rev_ind; cbn; eauto.
+  right; destruct IH as [-> | (? & ? & ->)].
+  exists []; eexists; reflexivity. 
+  do 2 eexists; reflexivity. 
+Qed.
+
+Ltac destruct_snoc xs :=
+  generalize (snoc_inv xs); intros [-> | (? & ? & ->)]. 
+
+Lemma prefix_snoc: forall {X: Type} (xs xs': list X) x,
+    xs' ⊑ snoc xs x ->
+    xs' = snoc xs x \/ xs' ⊑ xs.
+Proof.
+  induction xs as [| xs x' IH]; cbn; intros xs' x PRE.
+  - inv PRE; eauto.
+    inv H1; eauto.
+  - destruct xs'; auto.
+    inv PRE.
+    edestruct IH; eauto.
+    subst; eauto.
+Qed.
+
+Notation "x [[ n ]]" := (nth_error x n) (at level 12).
+
+(**************************** Utilites for predicates and relations **************************)
+
+Section Relations.
+
+  (**
+     Utilities to manipulates predicates and relations.
+     Should eventually be moved somewhere else.
+   *)
+  Section Pred.
+
+    Definition pred (A: Type) := A -> Prop.
+
+    Definition TT {A: Type}: pred A := fun _ => True.
+    Definition FF {A: Type}: pred A := fun _ => False.
+
+    Inductive Sum_Pred {A B: Type} (P1: pred A) (P2: pred B): pred (A + B) :=
+    | Sum_Pred_L: forall a, P1 a -> Sum_Pred P1 P2 (inl a) 
+    | Sum_Pred_R: forall b, P2 b -> Sum_Pred P1 P2 (inr b).
+
+    Inductive Inl_Pred {A B: Type} (P1: pred A): pred (A + B) :=
+    | Inl_PredC: forall a, P1 a -> Inl_Pred P1 (inl a).
+
+    Inductive Inr_Pred {A B: Type} (P2: pred B): pred (A + B) :=
+    | Inr_PredC: forall b, P2 b -> Inr_Pred P2 (inr b).
+
+    Definition Sub_Pred {A: Type} (P Q: pred A): Prop :=
+      forall a, P a -> Q a.
+
+  End Pred.
+
+  Section Rel.
+
+    Definition TT' {A: Type}: relation A := fun _ _ => True.
+    Definition FF' {A: Type}: relation A := fun _ _ => False.
+
+    Inductive Prod_Pred_to_Rel {A B: Type} (P1: A -> Prop) (P2: B -> Prop): A -> B -> Prop :=
+    | Prod_PredC: forall a b, P1 a -> P2 b -> Prod_Pred_to_Rel P1 P2 a b.
+
+    Inductive Sum_Rel {A B: Type} (R1: relation A) (R2: relation B): relation (A + B) :=
+    | Sum_Rel_L: forall a a', R1 a a' -> Sum_Rel R1 R2 (inl a) (inl a')
+    | Sum_Rel_R: forall b b', R2 b b' -> Sum_Rel R1 R2 (inr b) (inr b').
+
+    Inductive Join_Rel {A: Type} (R1 R2: relation A): relation A :=
+    | Join_Rel_L: forall a a', R1 a a' -> Join_Rel R1 R2 a a'
+    | Join_Rel_R: forall b b', R2 b b' -> Join_Rel R1 R2 b b'.
+
+  End Rel.
+
+End Relations.
+
+Infix "+'" := Sum_Pred (at level 40).
+Notation "'inl_' P" := (Inl_Pred P) (at level 5).
+Notation "'inr_' P" := (Inr_Pred P) (at level 5).
+Infix "->'" := (Prod_Pred_to_Rel) (at level 40).
+Infix "+''" := Sum_Rel (at level 40).
+Infix "∪" := Join_Rel (at level 60).
+Infix "⊆" := Sub_Pred (at level 60).
+Infix "⊆'" := inclusion (at level 60).
